Add sparse tr with sorry's

etch4/Etch/Verification/CodeGen/Sparse.lean
@@ -1,23 +1,48 @@
 import Etch.Verification.CodeGen.Translate
+import Etch.Verification.Semantics.Sparse
 
 namespace Etch.Verification
 section
 open Expr
 
-def SSparse (inds : ℕ) (vals : ℕ) : S ℕ ℤ where
+def SSparse (inds : ℕ) (vals : ℕ) (n : ℕ) : S ℕ ℤ where
   σ := Unit
   σ_enc := inferInstance
   Γ := fun _ => ℕ
   -- TODO: make a DSL to make it easier to write this code?
-  valid := lt (τ := ℕ) (var (by exact ())) (glb CType.nn inds)
+  valid := lt (τ := ℕ) (var (by exact ())) (glb CType.nn n)
   ready := op (.boolLit true) finZeroElim
   skip₀ := sorry
   skip₁ := sorry
   index := op .arrAccess ![glb (.lst .nn) inds, var (by exact ())]
   value := op .arrAccess ![glb (.lst .rr) vals, var (by exact ())]
-  init := .store (τ := ℕ) (.var (by exact ())) (op (.natLit 0) finZeroElim)
+  init := .store (.var (by exact ())) (0 : Expr _ ℕ)
+
+def SSparse.validInputs (inds : ℕ) (vals : ℕ) (n : ℕ) : Set GlobalVars :=
+{ g | List.Sorted (α := ℕ) (· ≤ ·) (g (.lst .nn) inds)
+      ∧ (g (.lst .nn) inds).length = g .nn n
+      ∧ (g (.lst .rr) vals).length = g .nn n }
+
+theorem SSparse.tr (inds : ℕ) (vals : ℕ) (n : ℕ) :
+    tr (SSparse.validInputs inds vals n) 
+      (fun g hg => Stream.sparseVec (ι := ℕ) ⟨g (.lst .nn) inds, hg.2.1⟩ ⟨g (.lst .rr) vals, hg.2.2⟩)
+      (SSparse inds vals n) := by
+  intros g hg
+  refine ⟨fun (q : ℕ) _ => q, ?_⟩
+  dsimp only
+  intro q
+  constructor
+  · simp [SSparse, Expr.lt_eval]; rfl
+  · sorry
+  · sorry
+  · sorry
+  · dsimp; sorry
+  · dsimp; sorry 
 
 end
+
+
+
 end Etch.Verification
 
 
