etch4/Etch/Verification/Semantics/Sparse.lean
@@ -1,4 +1,5 @@
 import Mathlib.Order.WellFoundedSet
+import Mathlib.Order.Basic
 import Etch.Verification.Semantics.SkipStream
 import Etch.Verification.Misc
 
@@ -26,18 +27,44 @@ def Stream.sparseVec (inds : Vector ι n) (vals : Vector α n) :
   σ := ℕ
   valid := fun i => i < n
   ready := fun i => i < n
-  skip := fun i _ jb => ((Fin.find fun k : Fin n => i ≤ k ∧ jb.1 ≤ inds.get k ∧ (jb.2 → jb.1 < inds.get k)).map Fin.val).getD n
+  skip := fun i hi jb => 
+    .find (p := fun k => i ≤ k ∧ ((hk : k < n) → jb < (inds.get ⟨k, hk⟩, true))) 
+      ⟨n, hi.le, fun hk => absurd hk (lt_irrefl n)⟩
+    --((Fin.find fun k : Fin n => i ≤ k ∧ jb.1 ≤ inds.get k ∧ (jb.2 → jb.1 < inds.get k)).map Fin.val).getD n
   index := fun i hi => inds.get ⟨i, hi⟩
   value := fun i hi => vals.get ⟨i, hi⟩
+
+lemma Stream.sparseVec_toOrder (inds : Vector ι n) (vals : Vector α n)
+  (q : (Stream.sparseVec inds vals).σ) (hq : Stream.valid _ q) :
+    (Stream.sparseVec inds vals).toOrder q hq = (inds.get ⟨q, hq⟩, true) := by
+  apply Prod.ext
+  · rfl
+  · simp [sparseVec, show (@LT.lt ℕ _ q n) from hq]
 
 attribute [reducible] Stream.sparseVec in
 theorem Stream.sparseVec_isBounded (inds : Vector ι n) (vals : Vector α n) :
     IsBounded (Stream.sparseVec inds vals) :=
-  IsBounded.mkWfSubset (· > ·) (Set.Finite.wellFoundedOn sorry) (by
-    rintro q hq ⟨j, b⟩; simp only [Stream.toOrder] at hq ⊢; simp
-    sorry
+  IsBounded.mkWfSubset (@GT.gt ℕ _) (Set.Finite.wellFoundedOn (α := ℕ) sorry) (by
+    rintro q hq jb; simp only [gt_iff_lt]
+    by_cases H : jb <ₗ toOrder (sparseVec inds vals) q hq
+    · right; refine ⟨H, ?_⟩
+      rw [Stream.sparseVec_toOrder] at H
+      simp only [Nat.find_eq_iff, le_refl, true_and, not_and, not_forall, not_lt]
+      constructor
+      · intro hk
+        convert H
+      · intros n h₁ h₂
+        exact absurd h₂ h₁.not_le
+    · left; rw [Stream.sparseVec_toOrder] at H
+      simp only [Nat.lt_find_iff, not_and, not_forall, not_lt]
+      intros m h₁ h₂
+      obtain rfl : m = q := le_antisymm h₁ h₂
+      exact ⟨hq, le_of_not_lt H⟩
+
+
+
+
+
   )
-
-
 
 end Etch.Verification
