etch4/Etch/Verification/CodeGen/Translate.lean
@@ -9,8 +9,8 @@ variable {ι α : Type _}
 structure tr₀ (s : Stream ι α) (t : S ι α) (ϕ : s.σ → Context (.ofσ t.Γ)) (q : s.σ) : Prop where
   (hvalid : s.valid q ↔ t.valid.eval (ϕ q))
   (hready : s.valid q → (s.ready q ↔ t.ready.eval (ϕ q)))
-  (hsk₀ : ∀ (i : ι), (h : s.valid q) → (ϕ (s.skip q h (i, ff))).vars = t.skip₀.eval (i ::ₐ ϕ q))
-  (hsk₁ : ∀ (i : ι), (h : s.valid q) → (ϕ (s.skip q h (i, tt))).vars = t.skip₁.eval (i ::ₐ ϕ q))
+  (hsk₀ : ∀ (i : ι), (h : s.valid q) → (ϕ (s.skip q h (i, false))).vars = t.skip₀.eval (i ::ₐ ϕ q))
+  (hsk₁ : ∀ (i : ι), (h : s.valid q) → (ϕ (s.skip q h (i, true))).vars = t.skip₁.eval (i ::ₐ ϕ q))
   (hind : (h : s.valid q) → s.index q h = t.index.eval (ϕ q))
   (hvalue : s.valid q → (h : s.ready q) → s.value q h = t.value.eval (ϕ q))
 
